\documentclass[12pt,a4paper]{article}
\usepackage[utf8]{inputenc}
\usepackage{amsmath}
\usepackage{amsfonts}
\usepackage{amssymb}
\usepackage{amsthm}

\begin{document}
\noindent
\textbf{Base:} Let $ y=\epsilon $ then $ |y|=0$
\begin{align*}
&\hat{\delta}(\hat{\delta}(q,x),y)		\tag{assumption}
\\ &=\hat{\delta}(\hat{\delta}(q,x),\epsilon)	\tag{definition}
\\ &=\hat{\delta}(q,x)					\tag{definition}
\\ &=\hat{\delta}(q,x\epsilon)			\tag{definition}
\\ &=\hat{\delta}(q,xy) 				\tag{assumption}
\\ &Q.E.D.
\end{align*}

\noindent
\textbf{IH:} if $|y|=n$ then $\hat{\delta}(q,x)=\hat{\delta}(\hat{\delta}(q,x),y)$\\

\noindent
\textbf{IS:} Assume the hypothesis is true for $n$. We will show that it is true for $n+1$ 
\noindent
Let $y=|za|$ where $z$ is a string such that $|z| \ge 0$ and $a$ is a character in $\Sigma$
\begin{align*}
&\hat{\delta}(\hat{\delta}(q,x),y)				\tag{assumption $y=za$}
\\ &= \hat{\delta}(\hat{\delta}(q,x),za) 		\tag{assumption}
\\ &= \delta(\hat{\delta}(\hat{\delta}(q,x),y),a) \tag{definition $\hat{\delta}$}
\\ &= \delta(\hat{\delta}(q,xz),a)				\tag{IH}
\\ &= \hat{\delta}(q,xza)						\tag{definition $\hat{\delta}$}
\\ &= \hat{\delta}(q,xy)						\tag{assumption $y=za$}
\\ &Q.E.D
\end{align*}

\begin{table}[h]
	\centering
	\begin{tabular}{|c|c|c|}
		\hline
		 & 0 & 1 \\
		\hline
		$\rightarrow$ p & \{q,s\} & $\emptyset$\\
		q & \{r\} & \{s\}\\
		r & $\emptyset$ & \{s\}\\
		*s & $\emptyset$ & $\emptyset$\\
		\hline
	\end{tabular}
\end{table}

\end{document}
